proof/SimMem.v
@@ -85,6 +85,8 @@ Module SimMem.
   (*   forall pr, sm0.(sim_val) (rs_src pr) (rs_tgt pr) *)
   (* . *)
 
+  Definition sim_regset `{SM: class} (sm0: SimMem.t) (rs_src rs_tgt: Asm.regset): Prop := forall pr, sm0.(sim_val) (rs_src pr) (rs_tgt pr).
+
   Inductive sim_args `{SM: class} (args_src args_tgt: Args.t) (sm0: SimMem.t): Prop :=
   | sim_args_Cstyle
       fptr_src vs_src m_src fptr_tgt vs_tgt m_tgt
@@ -94,7 +96,13 @@ Module SimMem.
       (VALS: sm0.(SimMem.sim_val_list) vs_src vs_tgt)
       (MEMSRC: m_src = sm0.(SimMem.src))
       (MEMTGT: m_tgt = sm0.(SimMem.tgt))
-  (* | sim_args_Asmstyle *)
+  | sim_args_Asmstyle
+      rs_src m_src rs_tgt m_tgt
+      (ASMSRC: args_src = Args.Asmstyle rs_src m_src)
+      (ASMTGT: args_tgt = Args.Asmstyle rs_tgt m_tgt)
+      (RS: sm0.(sim_regset) rs_src rs_tgt)
+      (MEMSRC: m_src = sm0.(SimMem.src))
+      (MEMTGT: m_tgt = sm0.(SimMem.tgt))
   .
 
   Inductive sim_retv `{SM: class} (retv_src retv_tgt: Retv.t) (sm0: SimMem.t): Prop :=
@@ -105,8 +113,18 @@ Module SimMem.
       (RETV: sm0.(SimMem.sim_val) v_src v_tgt)
       (MEMSRC: m_src = sm0.(SimMem.src))
       (MEMTGT: m_tgt = sm0.(SimMem.tgt))
-  (* | sim_retv_Asmstyle *)
+  | sim_retv_Asmstyle
+      rs_src m_src rs_tgt m_tgt
+      (ASMSRC: retv_src = Retv.Asmstyle rs_src m_src)
+      (ASMTGT: retv_tgt = Retv.Asmstyle rs_tgt m_tgt)
+      (RS: sm0.(sim_regset) rs_src rs_tgt)
+      (MEMSRC: m_src = sm0.(SimMem.src))
+      (MEMTGT: m_tgt = sm0.(SimMem.tgt))
   .
+
+  Lemma sim_args_sim_fptr `{SM: class}: forall sm0 args_src args_tgt (ARGS: sim_args args_src args_tgt sm0),
+      sm0.(sim_val) args_src.(Args.get_fptr) args_tgt.(Args.get_fptr).
+  Proof. i. inv ARGS; ss. Qed.
 
   Lemma sim_val_list_lepriv
         `{SM: class}
