backend/RenumberproofC.v
@@ -48,23 +48,19 @@ Proof.
   - eapply SoundTop.sound_state_local_preservation.
   - (* init bsim *)
     destruct sm_arg; ss. clarify.
-    inv SIMARGS; ss. clarify. inv INITTGT.
+    inv INITTGT. inv SIMARGS; ss; clarify.
     exploit make_match_genvs; eauto. { apply SIMSKENV. } intro SIMGE. des.
     eexists. eexists (SimMemId.mk _ _). esplits; eauto.
     + econs; eauto; ss.
       * inv TYP. rpapply match_callstates; eauto.
         { econs; eauto. }
         inv SAFESRC. folder. inv TYP.
-        exploit (Genv.find_funct_transf_genv SIMGE); eauto. rewrite <- FPTR in *. intro FINDFSRC; clarify.
-        ss. f_equal; try congruence.
+        exploit (Genv.find_funct_transf_genv SIMGE); eauto. intro FINDFSRC; clarify.
   - (* init progress *)
     des. inv SAFESRC. inv SIMARGS; ss.
     exploit make_match_genvs; eauto. { apply SIMSKENV. } intro SIMGE.
     exploit (Genv.find_funct_match_genv SIMGE); eauto. i; des. ss. clarify. folder.
-    inv TYP. esplits; eauto. econs; eauto.
-    + folder. rewrite <- FPTR. eauto.
-    + rewrite <- VALS. ss.
-    + ss. eauto with congruence.
+    inv TYP. esplits; eauto. econs; eauto. ss.
   - (* call wf *)
     inv MATCH; ss. destruct sm0; ss. clarify. inv CALLSRC. inv MATCHST; ss.
   - (* call fsim *)
@@ -80,14 +76,14 @@ Proof.
       * ss.
     + ss.
   - (* after fsim *)
-    inv AFTERSRC. inv SIMRET. ss. exists sm_ret. destruct sm_ret; ss. clarify.
+    inv AFTERSRC. inv SIMRET; clarify. ss. exists sm_ret. destruct sm_ret; ss. clarify.
     inv MATCH; ss. inv MATCHST; ss. esplits; eauto.
     + econs; eauto.
-    + econs; ss; eauto. destruct retv_src, retv_tgt; ss. clarify. econs; eauto.
+    + econs; ss; eauto. econs; eauto.
   - (* final fsim *)
     inv MATCH. inv FINALSRC; inv MATCHST; ss.
     inv STACKS; ss. destruct sm0; ss. clarify.
-    eexists (SimMemId.mk _ _). esplits; ss; eauto.
+    eexists (SimMemId.mk _ _). esplits; ss; eauto. econs; ss; eauto.
   - left; i. esplits; eauto.
     { apply modsem_receptive; et. }
     inv MATCH. ii. hexploit (@step_simulation prog skenv_link); eauto.
